{
 "cells": [
  {
   "attachments": {},
   "cell_type": "markdown",
   "metadata": {},
   "source": [
    "# Exercise 3\n",
    "Ole Gunnar Hovland, Jan Haakon Trabski and Alexander Hatle"
   ]
  },
  {
   "attachments": {},
   "cell_type": "markdown",
   "metadata": {},
   "source": [
    "# 1a)\n",
    "Discreticing the Black-Scholes equation and using Crank-Nicholson method."
   ]
  },
  {
   "attachments": {},
   "cell_type": "markdown",
   "metadata": {},
   "source": [
    "### Calculating the method\n",
    "Black-Scholes equation:\n",
    "$$\n",
    "u_{t}- \\frac{1}{2}\\sigma^{2}x^{2}u_{xx}-rxu_{x}+cu=f\n",
    "$$\n",
    "Discretizing using central differences in space, \n",
    "$$\n",
    "u_{t}- \\frac{1}{2}\\sigma^{2}x^{2} \\frac{1}{h^{2}}\\delta_{x}^{2}u-rx \\delta_{x,2h}u+cu=f\n",
    "$$\n",
    "setting $v_{m}(t)=u(x_{m},t)$\n",
    "$$\\dot v_{m}= \\frac{1}{2}\\sigma^{2}x_{m} \\frac{1}{h^{2}}(v_{m+1}-2v_{m}+v_{m-1})+rx_{m} \\frac{1}{2h}(v_{m+1}-v_{m-1})+f=: h(t,\\vec v)$$\n",
    "Crank-Nicholson scheme:\n",
    "$$\\vec y^{n+1}=\\vec y^{n}+ \\frac{k}{2}[h(t_{n},\\vec y^{n})+h(t_{n},y^{n+1})]$$\n",
    "We then get\n",
    "$$\\begin{align*}\n",
    "U^{n+1}_{m}=U^{n}_{m}+ \\frac{k}{2}\\Bigg[& \\left(\\frac{\\sigma^{2}}{2h^{2}}x_{m}^{2}+ \\frac{r}{2h}x_{m}\\right)(U_{m+1}^{n}+ U_{m+1}^{n+1})\\\\\n",
    "&-\\left(\\frac{\\sigma^{2}}{h^{2}}x_{m}^{2}+c\\right)(U_{m}^{n}+U_{m}^{n+1})\\\\\n",
    "&+ \\left(\\frac{\\sigma^{2}}{h^{2}}x_{m}^{2}- \\frac{r}{2h}x_{m}\\right)(U_{m-1}^{n}+U_{m-1}^{n+1})\\\\\n",
    "&+f(t_{n})+f(t_{n+1})\\Bigg]\n",
    "\\end{align*}$$\n",
    "Setting useful parameters \n",
    "$$\\alpha_{m}=\\frac{\\sigma^{2}k}{4h^{2}}x_{m}^{2},\\qquad \\beta_{m}=\\frac{rk}{4h}x_{m},\\qquad \\gamma=\\frac{ck}{2}\\qquad g(t_{n})= \\frac{k}{2}(f(t_{n}) + f(t_{n+1}))$$\n",
    "We end up with the system\n",
    "$$\\begin{align*}\n",
    "&(-\\alpha_{m}-\\beta_{m})U_{m+1}^{n+1}+(1+2\\alpha_{m}+\\gamma)U_{m}^{n+1}+(-\\alpha_{m}+\\beta_{m})U_{m-1}^{n+1}= \\\\\n",
    "\t&(\\alpha_{m}+\\beta_{m})U_{m+1}^{n}+(1-2\\alpha_{m}-\\gamma)U_{m}^{n}+(\\alpha_{m}-\\beta_{m})U_{m-1}^{n}+g(t_{n})\n",
    "\\end{align*}$$\n",
    "Or, in vector form\n",
    "$$A\\vec U^{n+1}+\\vec p^{n+1}=B\\vec U^{n}+\\vec q^{n}+\\vec{g^n}$$\n",
    "Where \n",
    "$$A=I_{M-1}+C,\\qquad B=I_{M-1}-C,\\qquad C=\\text{tridiag}(-\\alpha_{m}-\\beta_{m},2\\alpha)$$\n",
    "And vectors for the boundaries\n",
    "$$\\vec p^{n+1}= \\begin{bmatrix}(-\\alpha_{1}-\\beta_{1})U_{0}^{n+1} \\\\ 0 \\\\ \\vdots \\\\ 0 \\\\ (-\\alpha_{M-1}+\\beta_{M-1})U_{M}^{n+1}\\end{bmatrix}$$\n",
    "$$\\vec q^{n}= \\begin{bmatrix}(\\alpha_{1}+\\beta_{1})U_{0}^{n} \\\\ 0 \\\\ \\vdots \\\\ 0 \\\\ (\\alpha_{M-1}-\\beta_{M-1})U_{M}^{n}\\end{bmatrix}$$\n",
    "### Initial conditions and boundary conditions\n",
    "For now, we assume $f=0$\n",
    "#### European put\n",
    "$$u(x, 0)=\\text{max}(K-x,0)=:(K-x)^{+}\\tag{EP}$$\n",
    "For $K>0$. At $x=R$ we get\n",
    "$$u(R,t)=u(R,0)\\stackrel{R>K}{=} 0$$\n",
    "At $x=0$ we get a solvable ODE\n",
    "$$\\begin{align*}\n",
    "u_{t}+cu&=0\\\\\n",
    "u_{t}&= -cu\\\\\n",
    "\\text{(assume that) } u&=Ce^{-ct}\\\\\n",
    "\tu(0,0)\\stackrel{(EP)}{=}K \\quad\\Rightarrow\\quad C&= K \\\\\n",
    "u(0,t)=Ke^{-ct}\n",
    "\\end{align*}$$\n",
    "#### Binary call\n",
    "$$u(x,0)=\\text{sgn}^{+}(x-K)\\qquad \\text{sgn}^{+}(r)=\\begin{cases}\n",
    "0 & r<0 \\\\\n",
    "1 & r\\ge 0\n",
    "\\end{cases}$$\n",
    "Boundary at $x=R$\n",
    "$$u(R,t)=u(R,0)\\stackrel{R>K}{=}1$$\n",
    "We have the same ODE at $x=0$, but we get a different constant\n",
    "$$\\begin{align*}\n",
    "\tu&=C'e^{-ct}\\\\\n",
    "u(0,0)=0 \\quad\\Rightarrow\\quad u(0,t)&= 0\n",
    "\\end{align*}$$"
   ]
  },
  {
   "attachments": {},
   "cell_type": "markdown",
   "metadata": {},
   "source": [
    "## 1b)"
   ]
  },
  {
   "attachments": {},
   "cell_type": "markdown",
   "metadata": {},
   "source": [
    "\n",
    "\n",
    "We again have\n",
    "$$\\tag{BS} u_{t}- \\frac{1}{2}\\sigma^{2}x^{2}u_{xx}-r_{x}u_{x}+cu=0$$\n",
    "where $x\\in\\mathbb{R}^{+}$, $t\\in(0,\\text{T})$ , $\\sigma, r, c > 0$. Our boundryconditions are $u(R,t)=0$. \n",
    "\n",
    "We will use the same naming scheme for the methods as in a). Forward Euler, written in the same way as Crank-Nicolson in a), can be written as\n",
    "$$y^{n+1}=y^{n}+kf(t_{n}, y^{n})$$\n",
    "For our problem, in tandem with central difference, our problem can be discretized as \n",
    "$$\\begin{align*}\n",
    "U_{m}^{n+1}&=(\\alpha_{m}+\\beta_{m})U_{m+1}^{n}-(2\\alpha_{m}+\\gamma-1)U_{m}^{n}+(\\alpha_{m}-\\beta_{m})U_{m-1}^{n}\n",
    "\\end{align*}$$\n",
    "Using some helper-variables defined as\n",
    "$$\\begin{align*}\n",
    "\\alpha_{m}&:=\\frac{\\sigma^{2}x_{m}^{2}k}{2h^{2}},\\\\\n",
    "\\beta_{m}&:=\\frac{rx_{m}k}{2h},\\\\\n",
    "\\gamma&:=kc\n",
    "\\end{align*}$$\n",
    "Using the fact that $x_{m}=mh$ we can simplify further:\n",
    "$$\\begin{align*}\n",
    "\\alpha_{m}&:=\\frac{1}{2}\\sigma^{2}m^{2}k,\\\\\n",
    "\\beta_{m}&:=\\frac{1}{2}rmk,\\\\\n",
    "\\gamma&:=kc\n",
    "\\end{align*}$$\n",
    "To show monotonicity, we first want to reformulate our equation on the form\n",
    "$$-\\mathcal{L}_{h}U_p=f_{p}$$\n",
    "Where, in our case, $f_{p}= 0$. Rewriting our problem, in this form, we get\n",
    "$$-\\mathcal{L}_{h}U_p=U_{m}^{n+1}-(\\alpha_{m}+\\beta_{m})U_{m+1}^{n}-(1-2\\alpha_{m}-\\gamma)U_{m}^{n}-(\\alpha_{m}-\\beta_{m})U_{m-1}^{n}$$\n",
    "Now, there are a couple of things we have to show. (We'll use the definition of monotonicity from week 5, not 2) First we will have to demand coefficient positivity. For $(\\alpha_{m}+\\beta_{m})$ this is true since both $\\alpha_{m}$ and $\\beta_{m}$ are positive. Now for the third term:\n",
    "$$\\begin{align*}\n",
    "\\alpha_{m}-\\beta_{m}&\\geq0\\\\\n",
    "\\frac{1}{2}\\sigma^{2}m^{2}k-\\frac{1}{2}rmk&\\geq0\\\\\n",
    "\\frac{mk}{2}(\\sigma^{2}m-r)&\\geq0\n",
    "\\end{align*}$$\n",
    "since $m= 1,2,\\dots,M-1$ , $k>0$, and $\\sigma>r$, this inequality must allways be true. Now for showing non-negativity of the second term:\n",
    "$$\\begin{align*}\n",
    "1-2\\alpha_{m}-\\gamma&\\geq0\\\\\n",
    "1-\\sigma^{2}m^{2}k-kc&\\geq0\\\\\n",
    "1&\\geq k(\\sigma^{2}m^{2}+c)\n",
    "\\end{align*}$$\n",
    "Since $m\\leq M-1$ we get\n",
    "$$1\\geq k(\\sigma^{2}(M-1)^{2}+c)$$\n",
    "We'll call the last line above for CFL. Now, we need one last inequality fullfilled\n",
    "$$\\begin{align*}\n",
    "1&\\geq 1-\\sigma^{2}m^{2}k-kc+\\frac{1}{2}\\sigma^{2}m^{2}k-\\frac{1}{2}rmk+\\frac{1}{2}\\sigma^{2}m^{2}k+\\frac{1}{2}rmk \\\\\n",
    "0&\\geq-ck\\\\\n",
    "ck&\\geq0\n",
    "\\end{align*}$$\n",
    "This is always true.\n",
    "\n",
    "Now for Crank-Nicolson. Defining new helpervariables as\n",
    "$$\\begin{align*}\n",
    "\\alpha_{m}&:=\\frac{1}{4}\\sigma^{2}m^{2}k,\\\\\n",
    "\\beta_{m}&:=\\frac{1}{4}rmk,\\\\\n",
    "\\gamma&:=\\frac{kc}{2}\n",
    "\\end{align*}$$\n",
    "The CN method for our problem, written on the form $-\\mathcal{L}_{h}U_p=0$, is\n",
    "$$\\begin{align*}\n",
    "&-(\\alpha_{m}+\\beta_{m})U_{m+1}^{n+1}+(1+2\\alpha_m+\\gamma)U_{m}^{n+1}-(\\alpha_{m}-\\beta_{m})U_{m-1}^{n+1}\\\\\n",
    "&-(\\alpha_{m}+\\beta_{m})U_{m+1}^{n}-(1-2\\alpha_m-\\gamma)U_{m}^{n}-(\\alpha_{m}-\\beta_{m})U_{m-1}^{n}=0\n",
    "\\end{align*}$$\n",
    "Since we have so many coefficients, let us define some more helper variables!\n",
    "$$\\begin{align*}\n",
    "\\phi_{0}&=1+2\\alpha_{m}+\\gamma\\\\\n",
    "\\phi_{1}&=\\alpha_{m}+\\beta_{m}\\\\\n",
    "\\phi_{2}&=\\alpha_{m}-\\beta_{m}\\\\\n",
    "\\phi_{3}&=\\alpha_{m}+\\beta_{m}\\\\\n",
    "\\phi_{4}&=1-2\\alpha_{m}-\\gamma\\\\\n",
    "\\phi_{5}&=\\alpha_{m}-\\beta_{m}\\\\\n",
    "\\end{align*}$$\n",
    "The first property we will look at is that $\\phi_{0}\\geq \\sum\\limits_{i\\neq0}\\phi_{i}$ :\n",
    "$$\\begin{align*}\n",
    "1+2\\alpha_{m}+\\gamma\\geq&\\alpha_{m}+\\beta_{m}+\\alpha_{m}-\\beta_{m}+\\alpha_{m}\\\\\n",
    "&+\\beta_{m}+1-2\\alpha_{m}-\\gamma+\\alpha_{m}-\\beta_{m}\n",
    "\\end{align*}$$\n",
    "Now, many terms cancel out and we wnd up with\n",
    "$$\\gamma\\geq-\\gamma$$\n",
    "which is always true, since $\\gamma\\geq0$. Now we have to show that $\\phi_{i}\\geq0\\quad\\forall\\quad i$. We trivially see that $\\phi_{0},\\phi_{1},\\phi_{3}\\geq0$. We also see that $\\phi_{2}=\\phi_{5}=\\alpha_{m}-\\beta_{m}\\geq0$. \n",
    "$$\\begin{align*}\n",
    "\\Rightarrow\\quad \\alpha_{m}&\\geq\\beta_{m}\\\\\n",
    "\\frac{1}{4}\\sigma^{2}m^{2}k&\\geq \\frac{1}{4}rmk\\\\\n",
    "\\sigma^{2}m&\\geq r\n",
    "\\end{align*}$$\n",
    "This is allways true, since $m=1, 2,\\dots ,M-1$. Now, let us look at $\\phi_{4}$:\n",
    "$$\\begin{align*}\n",
    "\\phi_{4}=1-2\\alpha_{m}-\\gamma&\\geq0\\\\\n",
    "1-\\frac{1}{2}\\sigma^{2}m^{2}k- \\frac{kc}{2}&\\geq0\n",
    "\\end{align*}$$\n",
    "Rewriting, and using $m\\leq M-1$ we see that\n",
    "$$2\\geq k(\\sigma^{2}(M-1)^{2}+c)$$\n",
    "This is the CFL condition for Crank-Nicolson. \n",
    "\n",
    "Now we will show that Backward Euler (BE) is monotone if $\\sigma^{2}>r$. The method can be defined as\n",
    "$$y^{n+1}=y^{n}+kf(t_{n+1}, y^{n+1})$$\n",
    "For our problem, in tandem with central difference, our problem can be discretized as \n",
    "$$\\begin{align*}\n",
    "U_{m}^{n+1}&=U_{m}^{n}+(\\alpha_{m}+\\beta_{m})U_{m+1}^{n+1}-(2\\alpha_{m}+\\gamma)U_{m}^{n+1}+(\\alpha_{m}-\\beta_{m})U_{m-1}^{n+1}\n",
    "\\end{align*}$$\n",
    "Using the fact that $x_{m}=mh$ we define the helper variables\n",
    "$$\\begin{align*}\n",
    "\\alpha_{m}&:=\\frac{1}{2}\\sigma^{2}m^{2}k,\\\\\n",
    "\\beta_{m}&:=\\frac{1}{2}rmk,\\\\\n",
    "\\gamma&:=kc\n",
    "\\end{align*}$$\n",
    "Writing the scheme as $-\\mathcal{L}_{h}U_{p}=f_{p}=0$:\n",
    "$$\\begin{align*}\n",
    "-U_{m}^{n}-(\\alpha_{m}+\\beta_{m})U_{m+1}^{n+1}+(2\\alpha_{m}+\\gamma+1)U_{m}^{n+1}-(\\alpha_{m}-\\beta_{m})U_{m-1}^{n+1}=0\n",
    "\\end{align*}$$\n",
    "As we did with (CN) we define more helper variables:\n",
    "$$\\begin{align*}\n",
    "\\phi_{0}&=1+2\\alpha_{m}+\\gamma\\\\\n",
    "\\phi_{1}&=1\\\\\n",
    "\\phi_{2}&=\\alpha_{m}+\\beta_{m}\\\\\n",
    "\\phi_{3}&=\\alpha_{m}-\\beta_{m}\n",
    "\\end{align*}$$\n",
    "We trivially see that $\\phi_{0},\\phi_{1},\\phi_{2}\\geq0$. Now let us look at if $\\phi_{3}\\geq0$:\n",
    "$$\\begin{align*}\n",
    "\\alpha_{m}&\\geq\\beta_{m}\\\\\n",
    "\\frac{1}{2}\\sigma^{2}m^{2}k&\\geq\\frac{1}{2}rmk\\\\\n",
    "\\sigma^{2}m&\\geq r\n",
    "\\end{align*}$$\n",
    "Since $m=1, 2,\\dots ,M-1$ \n",
    "$$\\Rightarrow\\quad \\sigma^{2}\\geq r$$\n",
    "Which is allways true, since we have assumed $\\sigma^2>r$ . Now let us look at when $\\phi_{0}\\geq \\sum\\limits_{i\\neq0}\\phi_{i}$:\n",
    "$$\\begin{align*}\n",
    "1+2\\alpha_{m}+\\gamma&\\geq1+\\alpha_{m}+\\beta_{m}+\\alpha_{m}-\\beta_{m}\\\\\n",
    "\\gamma&\\geq0\\\\\n",
    "\\frac{ck}{2}&\\geq0\n",
    "\\end{align*}$$\n",
    "This is always true. \n",
    "$\\Rightarrow\\quad$ (BE), for our problem, will allways be monotone. $\\square$ "
   ]
  },
  {
   "attachments": {},
   "cell_type": "markdown",
   "metadata": {},
   "source": [
    "# 1c)"
   ]
  },
  {
   "cell_type": "markdown",
   "metadata": {},
   "source": []
  },
  {
   "attachments": {},
   "cell_type": "markdown",
   "metadata": {},
   "source": [
    "# 1d)"
   ]
  },
  {
   "cell_type": "markdown",
   "metadata": {},
   "source": []
  },
  {
   "attachments": {},
   "cell_type": "markdown",
   "metadata": {},
   "source": [
    "## 1e)"
   ]
  },
  {
   "attachments": {},
   "cell_type": "markdown",
   "metadata": {},
   "source": [
    "### Simple $u$\n",
    "We want to test CN in a setting where we know the exact solution $u(x,t)$. Let us start with a simple example.\n",
    "$$u(x,t)=(1+t)x^{2}$$\n",
    "Since this is a second-degree polynomial in space and time, CN will not have any error (except machine precision).\n",
    "The first thing we need to do is calculate the RHS $f$.\n",
    "$$\\begin{align*}\n",
    "u_{t}- \\frac{1}{2}\\sigma^{2}x^{2}u_{xx}-rxu_{x}+cu&=f\\tag{BS}\\\\\n",
    "\tx^{2}-\\sigma ^{2}x^{2}(1+t)+2r(1+t)x^{2}+c(1+t)&= f\\\\\n",
    "f=(1+t)x^{2}\\left( \\frac{1}{1+t}-\\sigma ^{2}+2r+c\\right)\n",
    "\\end{align*}$$\n",
    "IC and BCs\n",
    "$$\\begin{align*}\n",
    "u(x,0)&=x^{2}\\\\\n",
    "\tu(0,t)&=0\\\\\n",
    "u(R,t)&= R^{2}(1+t)\n",
    "\\end{align*}$$\n",
    "(insert plot here)\n",
    "\n",
    "### More complex $u$\n",
    "We choose\n",
    "$$u(x,t)=\\text{sin}\\left(\\frac{\\pi}{R}x\\right)e^{-t}$$\n",
    "Calculating $f$\n",
    "$$\\begin{align*}\n",
    "u_{t}- \\frac{1}{2}\\sigma^{2}x^{2}u_{xx}-rxu_{x}+cu&=f\\tag{BS}\n",
    "\\end{align*}$$\n",
    "$$\n",
    "\\begin{align*}\n",
    "-\\text{sin}\\left(\\frac{\\pi}{R}x\\right)- \\frac{1}{2}\\sigma^{2}x^{2} \\left(\\frac{\\pi}{R}\\right)^{2}\\left(-\\text{sin}\\left(\\frac{\\pi}{R}x\\right)\\right)&\\\\\n",
    "+ \\frac{rx\\pi}{R}\\left(\\text{cos}\\left(\\frac{\\pi}{R}x \\right)e^{-t}\\right)+c \\cdot\\text{sin}\\left(\\frac{\\pi}{R}x \\right)e^{-t}  &=f\\\\\n",
    "\t\tf=\\text{sin}\\left(\\frac{\\pi}{R}x \\right)e^{-t}\\left[-1+ \\frac{1}{2}\\left(\\frac{\\pi \\sigma x}{R} \\right)^{2}+c \\right] + \\frac{r \\pi x}{R}\\text{cos}\\left(\\frac{\\pi}{R}x \\right)e^{-t}\n",
    "\\end{align*}$$\n",
    "Boundary\n",
    "$$\\begin{align*}\n",
    "u(0,t) &= 0\\\\\n",
    "\tu(R,t) &= 0\\\\\n",
    "u(x,0)&= \\text{sin}\\left(\\frac{\\pi}{R}x \\right)\n",
    "\\end{align*}$$\n",
    "Okay, ready to plot the solution\n",
    "\n",
    "(insert numerical plot, analytical, and error plot here)\n",
    "\n",
    "Looks pretty good.\n",
    "\n",
    "Let's check the convergence rates\n",
    "\n",
    "(insert convergence plots here)\n",
    "\n",
    "As expected, we get (nearly) second order convergence in both space and time."
   ]
  },
  {
   "cell_type": "markdown",
   "metadata": {},
   "source": []
  }
 ],
 "metadata": {
  "kernelspec": {
   "display_name": "Python 3",
   "language": "python",
   "name": "python3"
  },
  "language_info": {
   "name": "python",
   "version": "3.8.2"
  },
  "orig_nbformat": 4,
  "vscode": {
   "interpreter": {
    "hash": "31f2aee4e71d21fbe5cf8b01ff0e069b9275f58929596ceb00d14d90e3e16cd6"
   }
  }
 },
 "nbformat": 4,
 "nbformat_minor": 2
}
